ver3_less_complex/Lemmas_bak.dfy
@@ -1,0 +1,350 @@
+include "Type.dfy"
+include "Auxilarily.dfy"
+include "System.dfy"
+include "Trace.dfy"
+
+module M_Lemma_bak {
+    import opened M_SpecTypes
+    import opened M_AuxilarilyFunc
+    import opened M_System
+    import opened M_Trace
+
+    // lemma{:axiom} Axiom_Byz_Constraints()
+    // ensures |Adversary_Nodes| <= f(|All_Nodes|)
+    // ensures Adversary_Nodes * Honest_Nodes == {}
+
+    // lemma{:axiom} Axiom_Common_Constraints()
+    // ensures All_Nodes != {}
+
+    lemma{:axiom} NoOuterClient()
+    ensures forall cert : Signature :: cert.Signature? ==> cert.signer in All_Nodes
+
+    lemma LemmaExistVoteMsgIfCertificateFormed(ss : SystemState)
+    requires ValidSystemState(ss)
+    ensures forall m : Msg | && m in ss.msgSent
+                             && ValidQC(m.justify)
+                          ::
+                             && (forall s : Signature | && s in m.justify.signatures
+                                                        && s.Signature?
+                                                     ::
+                                                        && (exists m : Msg | && m in ss.msgSent
+                                                                          ::
+                                                                             && m.partialSig.Signature?
+                                                                             && m.partialSig == s
+                                                            ) 
+                                )
+    // {
+
+    // }
+
+    lemma LemmaHonestNodeOnlyVoteOnceInOneView(ss : SystemState)
+    requires ValidSystemState(ss)
+    ensures forall m1 : Msg, m2 : Msg | && m1 in ss.msgSent
+                                        && m2 in ss.msgSent
+                                        && m1.partialSig.Signature?
+                                        && m2.partialSig.Signature?
+                                        && m1.partialSig.signer == m2.partialSig.signer
+                                        && IsHonest(ss, m1.partialSig.signer)
+                                        && m1.partialSig.mType == m2.partialSig.mType
+                                        && m1.partialSig.viewNum == m2.partialSig.viewNum
+                                      ::
+                                        m1.partialSig.block != m2.partialSig.block
+
+    // ensures forall s1 : Signature, s2 : Signature | 
+    //                                                 && s1.Signature?
+    //                                                 && s2.Signature?
+    //                                                 && s1.signer == s2.signer
+    //                                                 && IsHonest(ss, s1.signer)
+    //                                                 && s1.viewNum == s2.viewNum
+    //                                                 && s1.mType == s2.mType
+    //                                               ::
+    //                                                 s1.block == s2.block
+    {
+
+    }
+
+    /**
+     * Lemma: for 2 valid certificate, if they are conflict, then their coressponding view number should be different
+     */
+    lemma LemmaViewDiffOnConflictCertificatePrepare(ss : SystemState)
+    // requires All_Nodes != {}
+    requires ValidSystemState(ss)
+    ensures forall r1, r2, cert1, cert2 | && IsHonest(ss, r1)
+                                          && IsHonest(ss, r2)
+                                          && cert1 == ss.nodeStates[r1].prepareQC && cert1.Cert? 
+                                          && cert2 == ss.nodeStates[r2].prepareQC && cert2.Cert?
+                                          && cert1.block.Block?
+                                          && cert2.block.Block?
+                                          && !NoConflict(cert1.block, cert2.block)
+                                        ::
+                                          cert1.viewNum != cert2.viewNum
+
+    {
+
+        forall r1, r2, cert1, cert2 |   && IsHonest(ss, r1)
+                                        && IsHonest(ss, r2)
+                                        && cert1 == ss.nodeStates[r1].prepareQC && cert1.Cert? 
+                                        && cert2 == ss.nodeStates[r2].prepareQC && cert2.Cert?
+                                        && cert1.block.Block?
+                                        && cert2.block.Block?
+                                        && !NoConflict(cert1.block, cert2.block)
+
+        ensures cert1.viewNum != cert2.viewNum
+        {
+            // calc {
+            //     !NoConflict(cert1.block, cert2.block);
+            //     ==>
+            //     cert1.block != cert2.block;
+            // }
+            
+            var signers1 := getMajoritySignerInValidQC(cert1);
+            var signers2 := getMajoritySignerInValidQC(cert2);
+            LemmaTwoQuorumIntersection(All_Nodes, Adversary_Nodes, signers1, signers2);
+            // assert signers1 * signers2 * Honest_Nodes != {} by
+            // {
+            //     LemmaTwoQuorumIntersection(All_Nodes, Adversary_Nodes, signers1, signers2);
+            // }
+            // var replica :| replica in signers1 * signers2 * Honest_Nodes;
+            // var sign1 :| && sign1 in cert1.signatures
+            //              && sign1.signer == replica;
+            // var sign2 :| && sign2 in cert2.signatures
+            //              && sign2.signer == replica;
+            // assert sign1 != sign2;
+            // calc {
+            //     // sign1 != sign2
+            //     // ==>
+            //     cert1.viewNum != cert2.viewNum;
+            // }
+            // assert sign1.signer == sign2.signer;
+            // assert sign1.mType == sign2.mType;
+            // assert sign1.block != sign2.block;
+            // assert cert1.viewNum != cert2.viewNum by {
+            //     LemmaHonestNodeOnlyVoteOnceInOneView(ss);
+            // }
+            LemmaHonestNodeOnlyVoteOnceInOneView(ss);
+        }
+    } 
+
+    
+    /**
+     * Lemma: for 2 valid certificate, if they are conflict, then their coressponding view number should be different
+     */
+    lemma LemmaViewDiffOnConflictCertificate(ss : SystemState)
+    requires ValidSystemState(ss)
+    ensures forall m1, m2, cert1, cert2 |   && m1 in ss.msgSent
+                                            && m2 in ss.msgSent
+                                            && cert1 == m1.justify
+                                            && cert2 == m2.justify
+                                            && ValidQC(cert1)
+                                            && ValidQC(cert2)
+                                            && cert1.cType == cert2.cType
+                                            && cert1.block.Block?
+                                            && cert2.block.Block?
+                                            && !NoConflict(cert1.block, cert2.block)
+                                        ::
+                                            cert1.viewNum != cert2.viewNum
+    {
+        forall  m1, m2, cert1, cert2 |  && m1 in ss.msgSent
+                                        && m2 in ss.msgSent
+                                        && cert1 == m1.justify
+                                        && cert2 == m2.justify
+                                        && ValidQC(cert1)
+                                        && ValidQC(cert2)
+                                        && cert1.cType == cert2.cType
+                                        && cert1.block.Block?
+                                        && cert2.block.Block?
+                                        && !NoConflict(cert1.block, cert2.block)
+        ensures cert1.viewNum != cert2.viewNum
+        {
+            var signers1 := getMajoritySignerInValidQC(cert1);
+            var signers2 := getMajoritySignerInValidQC(cert2);
+            // LemmaTwoQuorumIntersection(All_Nodes, Adversary_Nodes, signers1, signers2);
+            assert signers1 * signers2 * Honest_Nodes != {} by
+            {
+                LemmaTwoQuorumIntersection(All_Nodes, Adversary_Nodes, signers1, signers2);
+            }
+            var replica :| replica in signers1 * signers2 * Honest_Nodes;
+            var sign1 :| && sign1 in cert1.signatures
+                         && sign1.signer == replica;
+            var sign2 :| && sign2 in cert2.signatures
+                         && sign2.signer == replica;
+            assert sign1 != sign2;
+            calc {
+                sign1 != sign2;
+                ==> { LemmaHonestNodeOnlyVoteOnceInOneView(ss);
+                      LemmaExistVoteMsgIfCertificateFormed(ss);
+                    }
+                cert1.viewNum != cert2.viewNum;
+            }
+        }
+    }
+
+    lemma LemmaMsgReceivedByReplicaIsSubsetOfAllMsgSentBySystem(ss : SystemState)
+    requires Reachable(ss)
+    ensures forall r, msgs | && IsHonest(ss, r)
+                             && msgs == ss.nodeStates[r].msgReceived
+                          ::
+                             && msgs <= ss.msgSent
+    {
+        forall r, msgs | && IsHonest(ss, r)
+                         && msgs == ss.nodeStates[r].msgReceived
+        ensures msgs <= ss.msgSent {
+            if SystemInit(ss) {
+                assert msgs <= ss.msgSent;
+            } else {
+                LemmaReachableStateIsValid(ss);
+                assert ValidSystemState(ss);
+            }
+        }
+    }
+
+    lemma LemmaExistValidPrepareQCForEveryValidPrecommitQC(ss : SystemState)
+    // requires ValidSystemState(ss)
+    requires Reachable(ss)
+    ensures forall m : Msg | && m in ss.msgSent
+                             && ValidQC(m.justify)
+                             && m.justify.cType == MT_PreCommit
+                          ::
+                             && (exists m2 : Msg :: && m2 in ss.msgSent
+                                                 && ValidQC(m2.justify)
+                                                 && m2.justify.cType == MT_Prepare
+                                                 && m2.justify.block == m.justify.block
+                                                 && m2.justify.viewNum == m.justify.viewNum
+                            )
+    // {
+
+    // }
+
+    lemma LemmaExistValidPrecommitQCForEveryValidCommitQC(ss : SystemState)
+    // requires ValidSystemState(ss)
+    requires Reachable(ss)
+    ensures forall m : Msg | && m in ss.msgSent
+                             && ValidQC(m.justify)
+                             && m.justify.cType == MT_Commit
+                          ::
+                             && (exists m2 : Msg :: && m2 in ss.msgSent
+                                                 && ValidQC(m2.justify)
+                                                 && m2.justify.cType == MT_PreCommit
+                                                 && m2.justify.block == m.justify.block
+                                                 && m2.justify.viewNum == m.justify.viewNum
+                            )
+    {
+
+    }
+
+
+    lemma LemmaExistValidPrepareQCForEveryValidCommitQC(ss : SystemState)
+    // requires ValidSystemState(ss)
+    requires Reachable(ss)
+    ensures forall m : Msg | && m in ss.msgSent
+                             && ValidQC(m.justify)
+                             && m.justify.cType == MT_Commit
+                          ::
+                             && (exists m2 : Msg :: && m2 in ss.msgSent
+                                                    // && m2.mType == MT_Prepare
+                                                    && ValidQC(m2.justify)
+                                                    && m2.justify.cType == MT_Prepare
+                                                    && m2.justify.block == m.justify.block
+                                                    && m2.justify.viewNum == m.justify.viewNum)
+    {
+        LemmaExistValidPrecommitQCForEveryValidCommitQC(ss);
+        LemmaExistValidPrepareQCForEveryValidPrecommitQC(ss);
+    }
+
+
+
+
+    lemma LemmaReplicaVotePrepareOnlyIfItRecievedASafetyPrepareQC(ss : SystemState, r : Address, lockedQC : Cert)
+    requires ValidSystemState(ss)
+    requires ValidQC(lockedQC)
+    requires IsHonest(ss, r)
+    ensures forall m : Msg | && m in ss.nodeStates[r].msgReceived
+                          :: 
+                            // && m.mType == MT_Prepare
+                            && m.partialSig.Signature?
+                            && m.partialSig.signer == r
+                            && m.partialSig.mType == MT_Prepare
+                            ==>
+                            (exists m1 : Msg :: && m1 in ss.nodeStates[r].msgReceived
+                                               && m1.mType == MT_Prepare
+                                               && ValidQC(m1.justify)
+                                               && m1.justify.cType == MT_Prepare
+                                               && m1.justify.viewNum > lockedQC.viewNum
+                                               && m1.block.Block?
+                                               && extension(m1.block, m1.justify.block)
+                                               && safeNode(m1.block, m1.justify, lockedQC)
+                                               && m.partialSig.block == m1.block
+                                               && m1.justify.viewNum < m.partialSig.viewNum
+                            )
+    
+    lemma LemmaVoteMsgInValidQCAlsoRecievedByVoter(ss : SystemState)
+    requires Reachable(ss)
+    ensures forall m : Msg | && m in ss.msgSent
+                             && ValidQC(m.justify)
+                          ::
+                            //  && var signers := getMajoritySignerInValidQC(m.justify)
+                             && var signatures := getVotesInValidQC(m.justify);
+                             && forall s | s in signatures
+                                        :: 
+                                          && (exists voteMsg : Msg :: 
+                                                                     && voteMsg in ss.nodeStates[s.signer].msgReceived
+                                                                     && voteMsg.partialSig == s)
+    // {}
+
+    lemma LemmaPrepareQCWithLowerViewIsExtensionOfPrepareQCWithHigherView(ss : SystemState)
+    requires Reachable(ss)
+    ensures forall m1, m2 : Msg | && m1 in ss.msgSent
+                                  && m2 in ss.msgSent
+                                  && ValidQC(m1.justify)
+                                  && ValidQC(m2.justify)
+                                  && m1.justify.cType == MT_Prepare
+                                  && m2.justify.cType == MT_Prepare
+                                  && m1.justify.viewNum <= m2.justify.viewNum
+                                ::
+                                  extension(m2.justify.block, m1.justify.block)
+    {
+        LemmaPrepareQCCanOnlyFormedByExtend(ss);
+    }
+    
+    lemma LemmaPrepareQCCanOnlyFormedByExtend(ss : SystemState)
+    // requires ValidSystemState(ss)
+    requires Reachable(ss)
+    ensures forall m : Msg | && m in ss.msgSent
+                             && ValidQC(m.justify)
+                             && m.justify.cType == MT_Prepare
+                          ::
+                             forall m_acs : Msg | && m_acs in ss.msgSent
+                                                  && ValidQC(m_acs.justify)
+                                                  && m_acs.justify.cType == MT_Prepare
+                                               ::
+                                                  m_acs.justify.viewNum <= m.justify.viewNum
+                                                  ==>
+                                                  extension(m.justify.block, m_acs.justify.block)
+    // {
+
+    // }
+                                                  
+
+    lemma LemmaReachableStateIsValid(ss : SystemState)
+    requires Reachable(ss)
+    ensures ValidSystemState(ss)
+    {
+        if !SystemInit(ss) {
+            var run : seq<SystemState> :|
+                                            && |run| > 1
+                                            && SystemInit(run[0])
+                                            && run[|run|-1] == ss
+                                            && (forall i | 0 <= i < |run|-1
+                                                        :: 
+                                                           && ValidSystemState(run[i])
+                                                           && SystemNext(run[i], run[i+1]));
+            forall i | 0 < i <= |run|-1
+            ensures ValidSystemState(run[i]) {
+                LemmaSystemTransitionHoldsValidity(run[i-1], run[i]);
+            }
+        } else {
+
+        }
+    }
+
+}
