ver3_less_complex/common/proofs.dfy
@@ -1,0 +1,20 @@
+module M_ProofTactic
+{
+    lemma LemmaSubsetTransitiveInSeq<T> (s : seq<set<T>>)
+    requires |s| > 0
+    requires forall i | 0 <= i < |s|-1 :: s[i] <= s[i+1]
+    ensures forall i | 0 <= i <= |s|-1 :: s[0] <= s[i]
+    {
+        forall i | 0 <= i <= |s|-1
+        ensures s[0] <= s[i] {
+            if i == 0 {
+
+            }
+            else
+            {
+                LemmaSubsetTransitiveInSeq(s[1..]);
+            }
+        }
+    }
+
+}
